Polish concurrency refinement and notation

examples/ConcChan.v
@@ -15,22 +15,37 @@ Section ConcChan.
 
   Notation config := (ConcStrategy.config ThreadState SharedState).
   Notation term := (ConcMonad.conc_term P).
+  Import ConcMonad.Notations.
+  Local Open Scope conc_scope.
+  #[local] Notation ret := (ConcMonad.ret (P:=P)).
 
-  Definition sender (ts : ThreadState) : term ThreadState := ConcMonad.ret ts.
-  Definition receiver (ts : ThreadState) : term ThreadState := ConcMonad.ret ts.
+  Definition sender (ch : Chan) (v : Val) (ts : ThreadState) : term ThreadState :=
+    ConcMonad.send (P:=P) ch v (fun _ => ret ts).
+
+  Definition receiver (ch : Chan) (ts : ThreadState) : term ThreadState :=
+    ConcMonad.recv (P:=P) ch (fun _ => ret ts).
 
   Definition compose_config (t1 t2 : ThreadState) (sh : SharedState) : config :=
     {| ConcStrategy.cfg_threads := [t1; t2];
        ConcStrategy.cfg_shared := sh |}.
 
+  Definition two_party_exchange (ch : Chan) (v : Val) (t1 t2 : ThreadState) (sh : SharedState) : term config :=
+    _ <- sender ch v t1;;
+    _ <- receiver ch t2;;
+    ret (compose_config t1 t2 sh).
+
   Definition R : term config -> config -> Prop := fun t c => ConcRefinement.R_conc P ThreadState SharedState t c.
 
   (** Placeholder correctness statement. *)
   Lemma chan_example_refines :
-    forall t1 t2 sh, R (ConcMonad.ret (compose_config t1 t2 sh)) (compose_config t1 t2 sh).
+    forall ch v t1 t2 sh, R (two_party_exchange ch v t1 t2 sh) (compose_config t1 t2 sh).
   Proof.
-    intros t1 t2 sh.
-    unfold R.
-    apply ConcRefinement.ret_refines.
+    intros ch v t1 t2 sh.
+    unfold two_party_exchange, R.
+    eapply (ConcRefinement.returns_bind P ThreadState SharedState) with (x:=t1).
+    - constructor. intro _. constructor.
+    - intro _. eapply (ConcRefinement.returns_bind P ThreadState SharedState) with (x:=t2).
+      + constructor. intro _. constructor.
+      + intro _. constructor.
   Qed.
 End ConcChan.
