models/ConcRefinement.v
@@ -11,33 +11,93 @@ Section ConcRefinement.
   Variable ThreadState SharedState : Type.
 
   Notation config := (ConcStrategy.config ThreadState SharedState).
+  Import ConcMonad.Notations.
+  Local Open Scope conc_scope.
+  Local Notation ret := (ConcMonad.ret (P:=P)).
+  Local Notation bind := (ConcMonad.bind (P:=P)).
+  Local Notation fmap := (ConcMonad.fmap (P:=P)).
 
-  (** A simple observational refinement: the concurrent term must be a pure return of [c]. *)
-  Definition R_conc (tm : ConcMonad.conc_term P config) (c : config) : Prop :=
-    exists c', tm = ConcMonad.ret (P:=P) c' /\ c' = c.
+  (** A simple total-correctness style refinement: every branch of the term returns [c]. *)
+  Inductive returns {X} : ConcMonad.conc_term P X -> X -> Prop :=
+  | returns_ret x : returns (ConcMonad.ret (P:=P) x) x
+  | returns_cons m k x : (forall a, returns (k a) x) -> returns (ConcMonad.Sig.cons m k) x.
+
+  Definition R_conc (tm : ConcMonad.conc_term P config) (c : config) : Prop := returns tm c.
 
   Lemma ret_refines (c : config) : R_conc (ConcMonad.ret (P:=P) c) c.
-  Proof. exists c; split; reflexivity. Qed.
+  Proof. constructor. Qed.
 
-  (** Spawn refinements hold trivially for the placeholder relation. *)
-  Lemma spawn_refinement :
-    forall (tid : ConcSignature.conc_tid P) (k : ConcSignature.conc_tid P -> ConcMonad.conc_term P config) (t : config),
-      R_conc (k tid) t ->
-      R_conc (ConcMonad.bind (P:=P) k (ConcMonad.ret (P:=P) tid)) t.
+  Lemma returns_bind {X Y} (t : ConcMonad.conc_term P X) (k : X -> ConcMonad.conc_term P Y)
+        (x : X) (y : Y) :
+    returns t x -> (forall x', returns (k x') y) -> returns (ConcMonad.bind (P:=P) k t) y.
   Proof.
-    intros tid k t H.
-    rewrite ConcMonad.ret_bind.
-    exact H.
+    revert k y.
+    induction 1; intros k y Hk; cbn.
+    - apply Hk.
+    - constructor. intro a. apply IHreturns. intro x0. apply Hk.
   Qed.
 
-  (** Yield refinements hold trivially for the placeholder relation. *)
+  Lemma returns_fmap {X Y} (f : X -> Y) (t : ConcMonad.conc_term P X) (x : X) :
+    returns t x -> returns (ConcMonad.fmap (P:=P) f t) (f x).
+  Proof.
+    induction 1; cbn.
+    - constructor.
+    - constructor. intro a. apply IHreturns.
+  Qed.
+
+  Lemma returns_tensor {X Y} (tx : ConcMonad.conc_term P X) (ty : ConcMonad.conc_term P Y) (x : X) (y : Y) :
+    returns tx x -> returns ty y -> returns (ConcMonad.tensor (P:=P) tx ty) (x, y).
+  Proof.
+    intros Hx Hy. unfold ConcMonad.tensor.
+    eapply returns_bind; eauto.
+    intro x0. eapply returns_bind; eauto. intro y0. constructor.
+  Qed.
+
+  (** Spawn and yield refinements propagate along all branches. *)
+  Lemma spawn_refinement :
+    forall (k : ConcSignature.conc_tid P -> ConcMonad.conc_term P config) (t : config),
+      (forall tid, R_conc (k tid) t) ->
+      R_conc (ConcMonad.spawn (P:=P) k) t.
+  Proof.
+    intros k t H.
+    unfold R_conc.
+    constructor. intro tid. apply H.
+  Qed.
+
   Lemma yield_refinement :
     forall (t : config) (k : unit -> ConcMonad.conc_term P config),
-      R_conc (k tt) t ->
-      R_conc (ConcMonad.bind (P:=P) k (ConcMonad.ret (P:=P) tt)) t.
+      (forall u, R_conc (k u) t) ->
+      R_conc (ConcMonad.yield (P:=P) k) t.
   Proof.
     intros t k H.
-    rewrite ConcMonad.ret_bind.
-    exact H.
+    unfold R_conc.
+    constructor. intro u. apply H.
+  Qed.
+
+  Lemma send_refinement :
+    forall (ch : ConcSignature.conc_chan P) (v : ConcSignature.conc_val P)
+           (k : unit -> ConcMonad.conc_term P config) (t : config),
+      (forall u, R_conc (k u) t) ->
+      R_conc (ConcMonad.send (P:=P) ch v k) t.
+  Proof.
+    intros ch v k t Hk. constructor. intro u. apply Hk.
+  Qed.
+
+  Lemma recv_refinement :
+    forall (ch : ConcSignature.conc_chan P)
+           (k : ConcSignature.conc_val P -> ConcMonad.conc_term P config) (t : config),
+      (forall v, R_conc (k v) t) ->
+      R_conc (ConcMonad.recv (P:=P) ch k) t.
+  Proof.
+    intros ch k t Hk. constructor. intro v. apply Hk.
+  Qed.
+
+  Lemma join_refinement :
+    forall (tid : ConcSignature.conc_tid P)
+           (k : ConcSignature.conc_val P -> ConcMonad.conc_term P config) (t : config),
+      (forall v, R_conc (k v) t) ->
+      R_conc (ConcMonad.join (P:=P) tid k) t.
+  Proof.
+    intros tid k t Hk. constructor. intro v. apply Hk.
   Qed.
 End ConcRefinement.
